simplification: PostMut is part of FnOnce, not FnMut

case_studies/tests/src/closures.rs
@@ -7,6 +7,7 @@
 // For the general form, we don't have syntactic sugar.
 #[rr::requires(#trait T::Pre := "λ _ _ _, True%I")]
 #[rr::requires(#trait T::Post := "λ _ _ _ ret, (∃ c : Z, ⌜ret = c⌝)%I")]
+#[rr::requires(#trait T::PostMut := "λ _ _ _ _ _, True%I")]
 //#[rr::require(#closure "T" : "True" -> "∃ c : Z, ret = c")]
 //#[rr::closure_computes("T", "λ _, c")]
 //#[rr::params("f" : "() → Z")]
@@ -24,6 +25,7 @@ fn closure_test_arg_fnonce_1<T>(x: T)
 #[rr::requires(#trait T::Pre := "λ _ _ x, ⌜x = -[42]⌝%I")]
 // TODO: allow to omit post
 #[rr::requires(#trait T::Post := "λ _ _ _ ret, True%I")]
+#[rr::requires(#trait T::PostMut := "λ _ _ _ _ _, True%I")]
 fn closure_test_arg_fnonce_2<T>(x: T)
     where T: FnOnce(i32) -> i32
 {
@@ -36,6 +38,7 @@ fn closure_test_arg_fnonce_2<T>(x: T)
 #[rr::verify]
 #[rr::requires(#trait T::Pre := "λ _ _ _, True%I")]
 #[rr::requires(#trait T::Post := "λ _ _ _ ret, True%I")]
+#[rr::requires(#trait T::PostMut := "λ _ _ _ _ _, True%I")]
 // TODO: allow this
 //#[rr::params("P")]
 //#[rr::requires(#trait T::Pre := "λ _ _, True%I")]
@@ -86,6 +89,7 @@ fn closure_test_arg_fnmut_1<T>(mut x: T)
 #[rr::verify]
 #[rr::requires(#trait T::Pre := "λ _ _ _, True%I")]
 #[rr::requires(#trait T::Post := "λ _ _ _ ret, True%I")]
+#[rr::requires(#trait T::PostMut := "λ _ _ _ _ _, True%I")]
 fn closure_test_call_fnonce_0<T>(x: T)
     where T: FnOnce() -> i32
 {
@@ -227,6 +231,7 @@ fn closure_test1() {
 #[rr::skip]
 #[rr::requires(#trait T::Pre := "λ _ _ _, True%I")]
 #[rr::requires(#trait T::Post := "λ _ _ _ ret, True%I")]
+#[rr::requires(#trait T::PostMut := "λ _ _ _ _ _, True%I")]
 fn closure_test8<T, U>(x: T, y: U)
     where U: FnOnce(T)
 {
@@ -346,6 +351,7 @@ fn closure_test3(y: &mut i32) {
 #[rr::skip]
 #[rr::requires(#trait T::Pre := "λ _ _ _, True%I")]
 #[rr::requires(#trait T::Post := "λ _ _ _ ret, True%I")]
+#[rr::requires(#trait T::PostMut := "λ _ _ _ _ _, True%I")]
 fn closure_test7<T, U>(x: T, y: U)
     where U: FnOnce(T)
 {
@@ -382,6 +388,7 @@ fn closure_test10() {
 #[rr::verify]
 #[rr::requires(#trait T::Pre := "λ _ _ _, True%I")]
 #[rr::requires(#trait T::Post := "λ _ _ _ ret, True%I")]
+#[rr::requires(#trait T::PostMut := "λ _ _ _ _ _, True%I")]
 fn closure_test_call_hrtb_1<T>(x: T)
     where T: for<'a> Fn(&'a i32) -> i32
 {
