rr_frontend/translation/src/traits/registry.rs
@@ -1112,7 +1112,6 @@ impl<'tcx, 'def> TR<'tcx, 'def> {
         if kind == ty::ClosureKind::FnOnce {
             attrs.insert("Pre".to_owned(), specs::traits::SpecAttrInst::Term(info.pre_encoded.clone()));
             attrs.insert("Post".to_owned(), specs::traits::SpecAttrInst::Term(info.post_encoded.clone()));
-        } else if kind == ty::ClosureKind::FnMut {
             attrs.insert(
                 "PostMut".to_owned(),
                 specs::traits::SpecAttrInst::Term(info.post_mut_encoded.clone().unwrap()),
