stdlib/closures/extra_specs.v
@@ -2,12 +2,20 @@
 Section extra_specs.
 Context `{RRGS : !refinedrustGS Σ}.
 Definition FnOnce_default_attrs {Self_rt Args_rt Output_rt : RT} : FnOnce_spec_attrs (RRGS:=RRGS) Self_rt Args_rt Output_rt :=
-  mk_FnOnce_spec_attrs (λ _ _ _ _, True%I) (λ _ _ _, True%I).
+  mk_FnOnce_spec_attrs (λ _ _ _ _, True%I) (λ _ _ _ _ _, True%I) (λ _ _ _, True%I).
 Definition FnMut_default_attrs {Self_rt Args_rt Output_rt : RT} :
   FnMut_spec_attrs (RRGS:=RRGS) Self_rt Args_rt Output_rt :=
-  mk_FnMut_spec_attrs (λ _ _ _ _ _, True%I). 
+  mk_FnMut_spec_attrs.
 Definition Fn_default_attrs {Self_rt Args_rt Output_rt : RT} :
   Fn_spec_attrs (RRGS:=RRGS) Self_rt Args_rt Output_rt :=
   mk_Fn_spec_attrs.
-
 End extra_specs.
+
+(*Global Arguments FnOnce_Post : simpl never.*)
+(*Global Typeclasses Opaque FnOnce_Post.*)
+
+(*Global Arguments FnOnce_Pre : simpl never.*)
+(*Global Typeclasses Opaque FnOnce_Pre.*)
+
+(*Global Arguments FnMut_PostMut : simpl never.*)
+(*Global Typeclasses Opaque FnMut_PostMut.*)
